theories/TM/Basic/Null.v
@@ -6,7 +6,7 @@ Section Mono_Nop.
 
   Variable sig : finType.
 
-  Definition NullTM : mTM sig 0 :=
+  Definition NullTM : TM sig 0 :=
     {|
       trans := fun '(q, s) => (q, Vector.nil _);
       start := tt;
